src/Implementations/FSParameters/FSParameters.v
@@ -1,0 +1,28 @@
+Require Import Framework.
+
+Axiom block_size: nat.
+Axiom disk_size: nat.
+
+Definition super_block_num := 0.
+Definition hdr_block_num := 1.
+Definition log_start := 2.
+Axiom log_length : nat.
+
+Definition data_start := 2 + log_length.
+Definition data_length := disk_size - data_start.
+
+(* Below all reside in data region *)
+(* For simplicity, it will be 1 inode per block *)
+Definition inode_blocks_start := data_start.
+Axiom inode_count: nat.
+Axiom inode_count_in_bounds: inode_count <= block_size.
+
+Definition file_blocks_start:= S(data_start + inode_count). (* 1 bitmap + inode_count inodes *)
+Axiom file_blocks_count : nat.
+Axiom file_blocks_count_in_bounds: file_blocks_count <= block_size.
+
+Axiom all_fits_to_data_region : 2 + inode_count + file_blocks_count <= data_length.
+
+Axiom addr_list_to_blocks : list addr -> list value.
+
+Global Opaque super_block_num hdr_block_num log_start data_start data_length inode_blocks_start file_blocks_start.
