src/Implementations/Log/LogParameters.v
@@ -1,5 +1,0 @@
-Require Import Primitives.
-
-Axiom hdr_block_num: addr.
-Axiom log_start : addr.
-Axiom log_length : nat.
